der_write_TL full proof

src/Lib/DWT/ExecDer_write_TL.v
@@ -5,18 +5,20 @@ Require Import ExecBer_tlv_tag_serialize
 
 Open Scope Z.
 
-Definition der_write_TL tag len size := 
+Definition der_write_TL tag len size constructed := 
   let (tl, t) := tag_serialize tag (Int.repr size) in
   let (ll, l) := length_serialize len (Int.repr (size - t)) in
-  let ls := tl ++ ll in
+  let ls := if eq_dec constructed 0%int 
+            then tl ++ ll 
+            else (upd_Znth 0 tl (Znth 0 tl or (Int.repr 32))%int) ++ ll in
   if ((t =? -1) || (32 <? t))%bool 
   then ([], -1)
   else if l =? -1 
-       then (ls, -1) 
+       then ([], -1) 
        else let s := l + t in
             if 32 <? s 
             then ([], -1)
-            else (tl ++ ll, s).
+            else (ls, s).
 
 Lemma tag_serialize_bounds : forall t l, -1 <= snd (tag_serialize t l) <= 6.
   { unfold tag_serialize.
@@ -34,23 +36,49 @@ Lemma length_serialize_bounds :
 Qed.
 
 Lemma der_write_TL_serialize_sum : 
-  forall t l s, 
+  forall t l s c, 
     let (tls, tl) := tag_serialize t (Int.repr s)  in
     let (lls, ll) := length_serialize l (Int.repr (s - tl)) in
     tl <> -1 ->
     ll <> -1 ->
     tl <= 32 ->
     tl + ll <= 32 ->
-    der_write_TL t l s = (tls ++ lls, tl + ll).
+    c = 0%int ->
+    der_write_TL t l s c = (tls ++ lls, tl + ll).
 Proof.
   intros.
   repeat break_let.
   unfold der_write_TL.
-  intros Z Z0 Z32 Zplus.
+  intros Z Z0 Z32 Zplus C.
   erewrite Heqp.
   erewrite Heqp0.
   repeat break_if; try destruct_orb_hyp;
   repeat Zbool_to_Prop; try nia.
+  intuition.
+  congruence.
+Qed.
+
+Lemma der_write_TL_serialize_sum_c : 
+  forall t l s c, 
+    let (tls, tl) := tag_serialize t (Int.repr s)  in
+    let (lls, ll) := length_serialize l (Int.repr (s - tl)) in
+    tl <> -1 ->
+    ll <> -1 ->
+    tl <= 32 ->
+    tl + ll <= 32 ->
+    c <> 0%int ->
+    der_write_TL t l s c = ((upd_Znth 0 tls (Znth 0 tls or (Int.repr 32))%int) ++ lls, tl + ll).
+Proof.
+  intros.
+  repeat break_let.
+  unfold der_write_TL.
+  intros Z Z0 Z32 Zplus C.
+  erewrite Heqp.
+  erewrite Heqp0.
+  repeat break_if; try destruct_orb_hyp;
+  repeat Zbool_to_Prop; try rep_omega.
+  erewrite e in C.
+  congruence.
   intuition.
 Qed.
 
