src/Lib/DWT/VSTder_write_TL.v
@@ -68,7 +68,7 @@ Definition der_write_TL_spec : ident * funspec :=
         valid_pointer cb)
   POST[tint]
     let size := if Val.eq cb nullval then 0 else 32 in
-    let (_, z) := der_write_TL tag l size in
+    let (_, z) := der_write_TL tag l size constructed in
     PROP() 
     LOCAL(temp ret_temp (Vint (Int.repr z)))
     SEP(func_ptr' dummy_callback_spec cb;
@@ -155,7 +155,7 @@ Proof.
         break_if;
           rewrite_if_b;
           reflexivity. }
-      assert (der_write_TL tag l 0 = ([], -1)) as L.
+      assert (der_write_TL tag l 0 constructed = ([], -1)) as L.
       { unfold der_write_TL.
         repeat break_let.
         inversion B.
@@ -167,10 +167,10 @@ Proof.
     + (* cb <> nullval *)
       unfold POSTCONDITION.
       unfold abbreviate.
-      destruct (der_write_TL tag l 32) as [ls z] eqn : DWT.
-      assert (fst (der_write_TL tag l 32) = ls) as FDWT by
+      destruct (der_write_TL tag l 32 constructed) as [ls z] eqn : DWT.
+      assert (fst (der_write_TL tag l 32 constructed) = ls) as FDWT by
              (unfold fst; break_let; inversion DWT; auto).
-      assert (snd (der_write_TL tag l 32) = z) as SDWT by
+      assert (snd (der_write_TL tag l 32 constructed) = z) as SDWT by
              (unfold snd; break_let; inversion DWT; auto).
       destruct (tag_serialize tag (Int.repr (32))) as [tl zt] eqn : TS. 
       destruct (length_serialize l (Int.repr (32 - zt))) as [ll zl] eqn : LS. 
@@ -209,7 +209,7 @@ Proof.
           try rep_omega; auto. }
         forward_if; try discriminate.
         forward.
-       assert (der_write_TL tag l 32 = ([], -1)) as K.
+       assert (der_write_TL tag l 32 constructed = ([], -1)) as K.
         { unfold der_write_TL.
           repeat break_let.
           cbn in Z.
@@ -257,211 +257,389 @@ Proof.
         1-2: ptrofs_compute_add_mul; try rep_omega.
         repeat forward.
         forward_if.
-        ** assert (zl = -1) as Z0. 
-           { eapply repr_inj_signed;
-               try rep_omega; subst; auto. }
-           assert (((zt =? -1) || (32 <? zt))%bool= false) as BC.
-           { eapply orb_false_intro;
-               Zbool_to_Prop; try nia. }
-           repeat forward.
-           entailer!. 
+      { assert (zl = -1) as Z0. 
+        { eapply repr_inj_signed;
+            try rep_omega; subst; auto. }
+        assert (((zt =? -1) || (32 <? zt))%bool= false) as BC.
+        { eapply orb_false_intro;
+            Zbool_to_Prop; try nia. }
+        repeat forward.
+        entailer!. 
+        unfold der_write_TL.
+        erewrite TS, LS.        
+        rewrite BC, Z0. auto.
+        erewrite LS.
+        rewrite_if_b.
+        erewrite sepcon_comm.
+        erewrite <- data_at_app_gen.
+        entailer!.
+        auto.
+        { subst; unfold default_val;
+            simpl;
+            try erewrite Zlength_list_repeat;
+            try nia; auto. }
+        nia.
+        reflexivity.
+        setoid_rewrite H4. 
+        unfold default_val.
+        simpl.
+        erewrite Zlength_list_repeat.                   
+        all: nia. }
+      { repeat forward.
+        forward_if.
+        ** remember (snd (tag_serialize tag (Int.repr 32))) as z0.
+           remember (snd (length_serialize l (Int.repr (32 - z0)))) as z1.
+           assert (zl <> -1) as Z0.
+           { eapply repr_neq_e. subst; auto. }
+           unfold POSTCONDITION.
+           unfold abbreviate.
+           rewrite <- SDWT.
            unfold der_write_TL.
-           erewrite TS, LS.        
-           rewrite BC, Z0. auto.
-           erewrite LS.
+           erewrite TS, LS.
+           replace ((zt =? -1) || (32 <? zt))%bool with false.              
+           replace (zl =? -1) with false.
+           replace (32 <? zl + zt) with true.
            rewrite_if_b.
+           forward.
+           entailer!.
+           subst.
            erewrite sepcon_comm.
+           change_compspecs CompSpecs.
            erewrite <- data_at_app_gen.
            entailer!.
            auto.
            { subst; unfold default_val;
                simpl;
                try erewrite Zlength_list_repeat;
-               try nia; auto. }
+               try nia; auto. } 
            nia.
            reflexivity.
-           setoid_rewrite H4. 
-           unfold default_val.
-           simpl.
-           erewrite Zlength_list_repeat.                   
-           all: nia. 
-         ** repeat forward.
-
-            forward_if.
-            ***
-              remember (snd (tag_serialize tag (Int.repr 32))) as z0.
-              remember (snd (length_serialize l (Int.repr (32 - z0)))) as z1.
-              assert (zl <> -1) as Z0.
-              { eapply repr_neq_e. subst; auto. }
-              unfold POSTCONDITION.
-              unfold abbreviate.
-              rewrite <- SDWT.
-              unfold der_write_TL.
-              erewrite TS, LS.
-              replace ((zt =? -1) || (32 <? zt))%bool with false.              
-              replace (zl =? -1) with false.
-              replace (32 <? zl + zt) with true.
-              rewrite_if_b.
-              forward.
-              entailer!.
-              subst.
-              erewrite sepcon_comm.
-              change_compspecs CompSpecs.
-              erewrite <- data_at_app_gen.
-              entailer!.
-              auto.
-              { subst; unfold default_val;
-                  simpl;
-                  try erewrite Zlength_list_repeat;
-                  try nia; auto. } 
-              nia.
-              reflexivity.
-              setoid_rewrite H5.
-              setoid_rewrite H11.
-              rep_omega.
-              symmetry.
-              Zbool_to_Prop; try rep_omega.
-              rewrite Int.unsigned_repr in *; try rep_omega.
-              symmetry.
-              Zbool_to_Prop. nia.
-              symmetry.
-              eapply orb_false_intro;
-                Zbool_to_Prop; try nia.            
-            *** 
-              erewrite LS.
-              erewrite SLS in *.
-              assert (zl <> -1) as Z0. 
-              { eapply repr_neq_e. auto. }
-              assert (0 < zt) as Zgt0.
-              { pose proof (tag_serialize_req_size_gt0 tag (Int.repr 32)).
-                erewrite TS in H3.
-                nia. }             
-              assert (0 < len tl) as LENTL.
-              { pose proof (tag_serialize_req_size tag (Int.repr 32)).
-                rewrite TS in H3.
-                erewrite H3.
-                all: nia. }
-              forward_if True; try congruence.
-        -- erewrite TLS in *. 
-           rewrite_if_b.
-           forward_if True.
-           erewrite TLL.
-           assert (zt = (len (map Vint tl))) as ZT.
-           { symmetry. 
-             pose proof (tag_serialize_req_size tag (Int.repr 32)).
-             erewrite TS in H5.
-             autorewrite with sublist.
-             eapply H5.
-             auto. }
-           erewrite ZT.           
-           erewrite split_data_at_sublist_tuchar with (j := 1%Z).
-           erewrite sublist_one with (lo := 0).
-           erewrite data_at_tuchar_singleton_array_eq.
-           Intros.
-           forward.
-           entailer!.
-           { unfold tag_serialize.
-             pose proof (Byte.Z_mod_modulus_range 
-                           (Int.unsigned (((tag & Int.repr 3) << Int.repr 6)
-                                            or (tag >>u Int.repr 2))%int)).
-             break_if.
-             rewrite if_false.
-             cbn.
-             erewrite Int.zero_ext_mod; try rep_omega.
-             erewrite <- Byte.Z_mod_modulus_eq;
-               rep_omega.
-             discriminate.
-             rewrite if_false by discriminate.
-             break_if;
-             cbn;
-             erewrite Int.zero_ext_mod; try rep_omega;
-              pose proof (Byte.Z_mod_modulus_range 
-                           ( Int.unsigned (((tag & Int.repr 3) << Int.repr 6)
-                                             or Int.repr 31)%int));
-             erewrite <- Byte.Z_mod_modulus_eq;
-               try rep_omega. }
-           forward.
-           rewrite <- ZT.
-           entailer!.
-           erewrite <- data_at_tuchar_singleton_array_eq.
-           erewrite <- data_at_app_gen.
-           entailer!.
-           1-10: autorewrite with sublist list norm;
-             autorewrite with sublist in ZT;
-             try rep_omega.
-           admit.
-           forward.
-           entailer!.
-           Intros.
-           forward_call ((Vptr b i), (zt + zl), app_key).
-           cbn in BT, BL.
-           rep_omega.
-           forward_if.
-           replace (zt + zl <? 0) with false in H4.
-           cbn in H4.
-           eapply typed_true_of_bool in H4.
-           eapply lt_inv in H4.
-           rewrite Int.signed_repr in H4.
-           autorewrite with norm in H4.
-           replace (Int.signed 0%int) with 0 in * by auto with ints.
-           rep_omega.
+           setoid_rewrite H5.
+           setoid_rewrite H11.
            rep_omega.
            symmetry.
-           Zbool_to_Prop.
-           cbn in BT, BL.
-           rewrite Int.unsigned_repr in *.
-           nia.
-           rep_omega.          
-           forward.
+           Zbool_to_Prop; try rep_omega.
+           rewrite Int.unsigned_repr in *; try rep_omega.
+           symmetry.
+           Zbool_to_Prop. nia.
+           symmetry.
+           eapply orb_false_intro;
+             Zbool_to_Prop; try nia.            
+        **
+          erewrite LS.
+          erewrite SLS in *.
+          assert (zl <> -1) as Z0. 
+          { eapply repr_neq_e. auto. }
+          assert (0 < zt) as Zgt0.
+          { pose proof (tag_serialize_req_size_gt0 tag (Int.repr 32)).
+            erewrite TS in H3.
+            nia. }             
+          assert (0 < len tl) as LENTL.
+          { pose proof (tag_serialize_req_size tag (Int.repr 32)).
+            rewrite TS in H3.
+            erewrite H3.
+            all: nia. }
+          forward_if
+     (PROP ( )
+     LOCAL (temp der_encoder._size (Vint (Int.repr zt + Int.repr (snd (ll, zl)))%int);
+     temp _tmp (Vint (Int.repr (snd (ll, zl)))); temp _t'5 (Vint (Int.repr (snd (ll, zl))));
+     temp _t'4 (Vint (Int.repr (32 - zt)));
+     temp _t'3 (Val.of_bool (Int.repr 32 < Int.repr zt)%int);
+     temp _buf_size (Vint (Int.repr 32)); temp der_encoder._t'1 (Vint (Int.repr 32));
+     lvar _buf (tarray tuchar 32) (Vptr b i); temp _tag (Vint tag); temp _len (Vint l);
+     temp _cb cb; temp _app_key app_key; temp _constructed (Vint constructed))
+     SEP (data_at Tsh (tarray tuchar (32 - zt))
+             (map Vint ll ++ sublist (len ll) (32 - zt) (default_val (tarray tuchar (32 - zt))))
+             (Vptr b (i + Ptrofs.repr zt)%ptrofs);
+      if Val.eq cb nullval 
+      then data_at Tsh (tarray tuchar (snd (tag_serialize tag (Int.repr 32))))
+       (map Vint (fst (tag_serialize tag (Int.repr 32)))) (Vptr b i)
+      else if eq_dec constructed 0%int 
+           then data_at Tsh (tarray tuchar (snd (tag_serialize tag (Int.repr 32))))
+                        (map Vint (fst (tag_serialize tag (Int.repr 32)))) (Vptr b i)
+ 
+           else  (data_at Tsh tuchar
+                         (Vint (Int.zero_ext 8 (Znth 0 tl or Int.repr 32)%int))
+                         (Vptr b i) *
+data_at Tsh (tarray tuchar (len (map Vint tl) - 1))
+    (sublist 1 (len (map Vint tl)) (map Vint tl)) (Vptr b (i + Ptrofs.repr 1)%ptrofs));
+     data_at_ Tsh enc_key_s app_key; valid_pointer cb; func_ptr' dummy_callback_spec cb))
+
+; try congruence.
+        -- erewrite TLS in *. 
            rewrite_if_b.
-           entailer!.
-        -- forward.
-           (* Exists (Vptr b i). *)
-           entailer!.
-           do 2 f_equal.
-           pose proof (der_write_TL_serialize_sum tag l 32) as N.
-           rewrite TS, LS in N.
-           erewrite N.
-           all: try rep_omega; auto.
-           rewrite if_false.
-           erewrite sepcon_comm.
-           change_compspecs CompSpecs. 
-           erewrite <- data_at_app_gen.
-           entailer!.
-           admit.
-           all: auto; try nia.
-           autorewrite with sublist list norm.
-           erewrite Zlength_sublist_correct.
-           all: try rep_omega.
-           admit.
-           unfold tarray.
-           erewrite Zlength_default_val_Tarray_tuchar.
-           nia.
-           nia.
-           (* replace (fst (der_write_TL tag l 32)) 
-              with (tl ++ ll).
-                assert ((fst (tag_serialize tag (Int.repr 32)) = tl)) as TLS
-          by (unfold fst; break_let; inversion TS; auto).
-                rewrite TLS.
-                erewrite map_app.
-                erewrite app_assoc.
-                f_equal.
-                admit.
-                admit. *)
-                
-                setoid_rewrite H5.
-                erewrite Zlength_app.
-                autorewrite with sublist.
-                erewrite Zlength_sublist_correct.
-                all: try rep_omega.
-                admit.
-                 {  subst; unfold default_val;
-                  simpl;
-                  try erewrite Zlength_list_repeat;
-                  try nia; auto. } 
-                 admit.
-                 
-                 ** admit. (* add lemma *)
-Admitted.
+           destruct (eq_dec constructed 0%int).            
+          { forward_if 
+             (PROP ( )
+  LOCAL (
+  temp der_encoder._size (Vint (Int.repr (len (map Vint tl)) + Int.repr (snd (ll, zl)))%int);
+  temp _tmp (Vint (Int.repr (snd (ll, zl)))); temp _t'5 (Vint (Int.repr (snd (ll, zl))));
+  temp _t'4 (Vint (Int.repr (32 - len (map Vint tl))));
+  temp _t'3 (Val.of_bool (Int.repr 32 < Int.repr (len (map Vint tl)))%int);
+  temp _buf_size (Vint (Int.repr 32)); temp der_encoder._t'1 (Vint (Int.repr 32));
+  lvar _buf (tarray tuchar 32) (Vptr b i); temp _tag (Vint tag); temp _len (Vint l); 
+  temp _cb cb; temp _app_key app_key; temp _constructed (Vint constructed))
+  SEP (data_at Tsh (tarray tuchar (32 - len (map Vint tl)))
+         (map Vint ll ++
+          sublist (len ll) (32 - len (map Vint tl))
+            (default_val (tarray tuchar (32 - len (map Vint tl)))))
+         (Vptr b (i + Ptrofs.repr (len (map Vint tl)))%ptrofs);
+ data_at Tsh (tarray tuchar (len (map Vint tl)))
+  (map Vint tl) (Vptr b i);
+  data_at_ Tsh enc_key_s app_key; valid_pointer cb; func_ptr' dummy_callback_spec cb)); 
+try congruence.
+            erewrite TLL.
+            assert (zt = (len (map Vint tl))) as ZT.
+            { symmetry. 
+              pose proof (tag_serialize_req_size tag (Int.repr 32)).
+              erewrite TS in H5.
+              autorewrite with sublist.
+              eapply H5.
+              auto. }
+            erewrite ZT.           
+            forward.
+            entailer!.
+            repeat rewrite_if_b.
+            assert (zt = (len (map Vint tl))) as ZT.
+            { symmetry. 
+              pose proof (tag_serialize_req_size tag (Int.repr 32)).
+              erewrite TS in H4.
+              autorewrite with sublist.
+              eapply H4.
+              auto. }
+            erewrite <- ZT.
+            unfold snd.
+            forward_call ((Vptr b i), (zt + zl), app_key).
+            cbn in BT, BL.
+            rep_omega.
+            forward_if.
+            replace (zt + zl <? 0) with false in H4.
+            cbv in H4.
+            congruence.
+            symmetry.
+            Zbool_to_Prop.
+            cbn in BT, BL.
+            rewrite Int.unsigned_repr in *.
+            nia.
+            rep_omega.          
+            forward.
+            rewrite_if_b.
+            entailer!. }
+ { forward_if 
+             (PROP ( )
+  LOCAL (temp _t'7 (Vint (Znth 0 tl));
+  temp der_encoder._size (Vint (Int.repr (len (map Vint tl)) + Int.repr (snd (ll, zl)))%int);
+  temp _tmp (Vint (Int.repr (snd (ll, zl)))); temp _t'5 (Vint (Int.repr (snd (ll, zl))));
+  temp _t'4 (Vint (Int.repr (32 - len (map Vint tl))));
+  temp _t'3 (Val.of_bool (Int.repr 32 < Int.repr (len (map Vint tl)))%int);
+  temp _buf_size (Vint (Int.repr 32)); temp der_encoder._t'1 (Vint (Int.repr 32));
+  lvar _buf (tarray tuchar 32) (Vptr b i); temp _tag (Vint tag); temp _len (Vint l); 
+  temp _cb cb; temp _app_key app_key; temp _constructed (Vint constructed))
+  SEP (data_at Tsh (tarray tuchar (32 - len (map Vint tl)))
+         (map Vint ll ++
+          sublist (len ll) (32 - len (map Vint tl))
+            (default_val (tarray tuchar (32 - len (map Vint tl)))))
+         (Vptr b (i + Ptrofs.repr (len (map Vint tl)))%ptrofs);
+data_at Tsh tuchar (Vint (Int.zero_ext 8 (Znth 0 tl or Int.repr 32)%int)) (Vptr b i);
+data_at Tsh (tarray tuchar (len (map Vint tl) - 1))
+    (sublist 1 (len (map Vint tl)) (map Vint tl)) (Vptr b (i + Ptrofs.repr 1)%ptrofs);
 
+  data_at_ Tsh enc_key_s app_key; valid_pointer cb; func_ptr' dummy_callback_spec cb));
+     try congruence.
+   erewrite TLL.
+   assert (zt = (len (map Vint tl))) as ZT.
+   { symmetry. 
+     pose proof (tag_serialize_req_size tag (Int.repr 32)).
+     erewrite TS in H5.
+     autorewrite with sublist.
+     eapply H5.
+     auto. }
+   erewrite ZT.    
+   erewrite split_data_at_sublist_tuchar with (j := 1%Z).
+   erewrite sublist_one with (lo := 0).
+   erewrite data_at_tuchar_singleton_array_eq.
+   Intros.
+   forward.
+   entailer!.
+   { unfold tag_serialize.
+     pose proof (Byte.Z_mod_modulus_range 
+                   (Int.unsigned (((tag & Int.repr 3) << Int.repr 6)
+                                    or (tag >>u Int.repr 2))%int)).
+     break_if.
+     rewrite if_false.
+     cbn.
+     erewrite Int.zero_ext_mod; try rep_omega.
+     erewrite <- Byte.Z_mod_modulus_eq;
+       rep_omega.
+     discriminate.
+     rewrite if_false by discriminate.
+     break_if;
+       cbn;
+       erewrite Int.zero_ext_mod; try rep_omega;
+         pose proof (Byte.Z_mod_modulus_range 
+                       ( Int.unsigned (((tag & Int.repr 3) << Int.repr 6)
+                                         or Int.repr 31)%int));
+         erewrite <- Byte.Z_mod_modulus_eq;
+         try rep_omega. }
+   forward.
+   rewrite <- ZT.
+   repeat rewrite_if_b.
+   entailer!.
+   autorewrite with sublist list norm.
+   autorewrite with sublist in ZT.
+   rewrite ZT.
+   entailer!.
+   1-5: auto; autorewrite with sublist in *;
+     unfold snd in *; try nia.   
+   assert (zt = (len (map Vint tl))) as ZT.
+   { symmetry. 
+     pose proof (tag_serialize_req_size tag (Int.repr 32)).
+     erewrite TS in H4.
+     autorewrite with sublist.
+     eapply H4.
+     auto. }
+   erewrite <- ZT.
+   unfold snd.
+   unfold POSTCONDITION.
+   unfold abbreviate.
+   unfold MORE_COMMANDS.
+   unfold abbreviate.
+   forward_call ((Vptr b i), (zt + zl), app_key).
+   cbn in BT, BL.
+   rep_omega.
+   forward_if.
+   replace (zt + zl <? 0) with false in H4.
+   cbv in H4.
+   congruence.
+   symmetry.
+   Zbool_to_Prop.
+   cbn in BT, BL.
+   rewrite Int.unsigned_repr in *.
+   nia.
+   rep_omega.
+   forward.
+   rewrite_if_b.
+   rewrite ZT.
+   entailer!. }
+        --
+          
+          forward.
+          destruct (eq_dec constructed 0%int).
+          pose proof (der_write_TL_serialize_sum tag l 32) as N.             
+          rewrite TS, LS in N.
+          erewrite N.
+          repeat rewrite_if_b.
+          entailer!.
+          remember (snd (tag_serialize tag (Int.repr 32))) as zt.
+          remember (snd (length_serialize l (Int.repr (32 - zt)))) as zl.
+          remember (fst (tag_serialize tag (Int.repr 32))) as tl.
+          remember (fst (length_serialize l (Int.repr (32 - zt)))) as ll.
+          assert (zl = len ll) as ZL.
+          { symmetry. 
+            pose proof (length_serialize_req_size l (Int.repr (32 - zt))).
+            erewrite LS in *.
+            auto. }
+          rewrite <- ZL.
+          erewrite sepcon_comm.
+          erewrite <- data_at_app_gen.
+          entailer!.
+          all: autorewrite with sublist; try  erewrite ZL; auto; try nia.
+          assert (zt = len tl) as ZT.
+          { symmetry. 
+            pose proof (tag_serialize_req_size tag (Int.repr (32))).
+            erewrite TS in *.
+            auto. }
+          auto.
+          autorewrite with sublist in H5.
+          auto.
+          erewrite Zlength_sublist_correct.
+          assert (zt = len tl) as ZT.
+          { symmetry. 
+            pose proof (tag_serialize_req_size tag (Int.repr (32))).
+            erewrite TS in *.
+            auto. }
+          rep_omega.
+          unfold snd in *.
+          nia.
+          unfold tarray.
+          erewrite Zlength_default_val_Tarray_tuchar; nia. 
+          auto with ints.
 
+          pose proof (der_write_TL_serialize_sum_c tag l 32) as N.             
+          rewrite TS, LS in N.
+          erewrite N.
+          repeat rewrite_if_b.
+          entailer!.
+          
+          remember (snd (tag_serialize tag (Int.repr 32))) as zt.
+          remember (snd (length_serialize l (Int.repr (32 - zt)))) as zl.
+          remember (fst (tag_serialize tag (Int.repr 32))) as tl.
+          remember (fst (length_serialize l (Int.repr (32 - zt)))) as ll.
+
+          assert (zt = len tl) as ZT.
+          { symmetry. 
+            pose proof (tag_serialize_req_size tag (Int.repr (32))).
+            erewrite TS in *.
+            auto. }
+          assert (zl = len ll) as ZL.
+          { symmetry. 
+            pose proof (length_serialize_req_size l (Int.repr (32 - zt))).
+            erewrite LS in *.
+            auto. }
+          rewrite <- ZL.
+          erewrite sepcon_comm.
+          erewrite <- data_at_tuchar_singleton_array_eq.
+          erewrite sepcon_comm.
+          erewrite sepcon_assoc.
+          erewrite <- data_at_app_gen with (ls := Vint (Int.zero_ext 8 (Znth 0 tl or Int.repr 32)%int)
+                                                      :: (sublist 1 (len tl) (map Vint tl))).
+          erewrite sepcon_comm.
+          erewrite <- data_at_app_gen.
+          entailer!.
+          all: autorewrite with sublist; try  erewrite ZL; auto; try nia.
+          auto.
+          autorewrite with sublist in H5.
+          auto.
+          erewrite Zlength_sublist_correct.
+          rep_omega.
+          unfold snd in *.
+          nia.
+          unfold tarray.
+          erewrite Zlength_default_val_Tarray_tuchar; nia. }
+      all: try erewrite TLL.
+      assert (zt = len tl) as ZT.
+      { symmetry. 
+        pose proof (tag_serialize_req_size tag (Int.repr (32))).
+        erewrite TS in *.
+        auto. }
+      auto.
+
+      unfold tarray.
+      { subst; unfold default_val;
+          simpl;
+          try erewrite Zlength_list_repeat;
+          try nia; auto. }
+      Focus 2.
+      assert (zt = len tl) as ZT.
+      { symmetry. 
+        pose proof (tag_serialize_req_size tag (Int.repr 32)).
+        erewrite TS in *.
+        auto. }
+      unfold default_val;
+        simpl;
+        try erewrite Zlength_list_repeat;
+        try nia; auto.
+      assert (zt = len tl) as ZT.
+      { symmetry. 
+        pose proof (tag_serialize_req_size tag (Int.repr 32)).
+        erewrite TS in *.
+        auto. }
+      
+      erewrite ZT.
+      autorewrite with sublist list norm.
+      f_equal.
+      unfold default_val.
+      simpl.
+      erewrite <- sublist_list_repeat with (k := 32); auto; nia.
+      nia.
+Qed.
